theory/System/PathORAMDef.v
@@ -322,10 +322,6 @@ Section PORAM.
   Definition kv_rel (id : block_id) (v : nat) (st : state) : Prop :=
     (blk_in_stash id v st) \/ (blk_in_path id v st).
 
-  Definition kv_rel2 (id : block_id) (v : nat) (st : state) : Prop :=
-    ((blk_in_stash id v st) \/ (blk_in_path id v st)) \/
-      ((not ((blk_in_stash id v st) \/ (blk_in_path id v st))) /\ (v = O)).
-       
   Definition locate_node_in_tr (o : oram) (lvl : nat) (p : path) : option bucket :=
     match lookup_tree o lvl p with
     | None => None
